Coll toMultiset

Algorithm/Data/Classes/Collection.lean
@@ -3,41 +3,52 @@ Copyright (c) 2023 Yuyang Zhao. All rights reserved.
 Released under Apache 2.0 license as described in the file LICENSE.
 Authors: Yuyang Zhao
 -/
-import Mathlib.Data.List.Basic
+import Mathlib.Data.Multiset.Basic
 
 class Collection (C : Type*) (α : outParam Type*) where
-  size : C → Nat
   empty : C
+  toMultiset : C → Multiset α
   isEmpty : C → Bool
-  isEmpty_empty : isEmpty empty
-  size_eq_zero_iff c : size c = 0 ↔ isEmpty c
---TODO: toMultiset
---TODO: `size` for fixed size DS?
+  size : C → Nat
+  card_toMultiset_eq_size c : Multiset.card (toMultiset c) = size c
+  toMultiset_empty : toMultiset empty = 0
+  isEmpty_iff_size_eq_zero c : isEmpty c ↔ size c = 0
+
+attribute [simp] Collection.card_toMultiset_eq_size
 
 section
 variable {α : Type*}
 
 instance : Collection (List α) α where
-  size := List.length
   empty := []
+  toMultiset := (↑)
+  size := List.length
+  card_toMultiset_eq_size c := rfl
   isEmpty := List.isEmpty
-  isEmpty_empty := rfl
-  size_eq_zero_iff l := by cases l <;> (simp; rfl)
+  toMultiset_empty := rfl
+  isEmpty_iff_size_eq_zero l := by cases l <;> (simp; rfl)
 
 instance : Collection (Array α) α where
-  size := Array.size
   empty := #[]
+  toMultiset a := ↑a.toListRev
+  size := Array.size
+  card_toMultiset_eq_size c := by simp
   isEmpty := Array.isEmpty
-  isEmpty_empty := rfl
-  size_eq_zero_iff l := by simp
-
-end
+  toMultiset_empty := rfl
+  isEmpty_iff_size_eq_zero l := by simp
 
 namespace Collection
 variable {C α : Type*} [Collection C α] (c : C)
 
+instance (priority := 100) : Membership α C where
+  mem a c := a ∈ toMultiset c
+
+lemma isEmpty_empty : isEmpty (empty : C) := by
+  rw [isEmpty_iff_size_eq_zero, ← card_toMultiset_eq_size, toMultiset_empty]
+  rfl
+
 lemma isEmpty_eq_decide_size : isEmpty c = decide (size c = 0) := by
-  simp only [size_eq_zero_iff, Bool.decide_coe]
+  simp only [← isEmpty_iff_size_eq_zero, Bool.decide_coe]
 
 lemma isEmpty_eq_size_beq_zero : isEmpty c = (size c == 0) := by
   rw [isEmpty_eq_decide_size]
